{
 "cells": [
  {
   "cell_type": "markdown",
   "id": "67c42cab-ec16-46d6-8f54-14c2a8300e06",
   "metadata": {},
   "source": [
    "# Problem Set 0"
   ]
  },
  {
   "cell_type": "markdown",
   "id": "4093cafd-7a24-498e-ae17-1d0dba59b25c",
   "metadata": {},
   "source": [
    "1\n",
    "\n",
    "(a)\n",
    "$$f(x) = \\frac{1}{2}x^T A x + b^T x = \\frac{1}{2} \\sum_{i=1}^n \\sum_{j=1}^n x_i A_{ij} x_j + \\sum_{i=1}^n b_i x_i$$\n",
    "$$\n",
    "\\begin{align}\n",
    "\\frac{\\partial}{\\partial x_k} f(x) \n",
    "&= \\frac{1}{2} \\sum_{i=1}^n \\sum_{j=1}^n (\\delta_{ik} A_{ij} x_j + x_i A_{ij} \\delta_{jk}) + \\sum_{i=1}^n b_i \\delta_{ik}\n",
    "\\\\\n",
    "&= \\frac{1}{2} (\\sum_{j=1}^n A_{kj} x_j + \\sum_{i=1}^n x_i A_{ik}) + b_k\n",
    "\\\\\n",
    "&= \\frac{1}{2} (\\sum_{j=1}^n A_{kj} x_j + \\sum_{i=1}^n A_{ki} x_i) + b_k\n",
    "\\\\\n",
    "&= \\frac{1}{2} (\\sum_{j=1}^n A_{kj} x_j + \\sum_{i=1}^n A_{ki} x_i) + b_k\n",
    "\\\\\n",
    "&=\\sum_{i=1}^n A_{ki} x_i + b_k\n",
    "\\\\\n",
    "&=(A x)_k + b_k\n",
    "\\end{align}\n",
    "$$\n",
    "So \n",
    "$$\\nabla f(x) = Ax + b$$\n",
    "\n",
    "(b)\n",
    "$$\\frac{\\partial}{\\partial x_k} f(x) = g'(h(x))\\frac{\\partial h(x)}{\\partial x_k}$$\n",
    "\n",
    "So\n",
    "\n",
    "$$ \\nabla f(x) = g'(h(x)) \\nabla h(x)$$\n",
    "\n",
    "(c)\n",
    "\n",
    "$$\\frac{\\partial^2}{\\partial x_i \\partial x_j} f(x) = \\frac{1}{2} \\frac{\\partial^2}{\\partial x_i \\partial x_j} \\sum_{k=1}^n \\sum_{l=1}^n x_k A_{kl} x_l$$\n",
    "\n",
    "Only two terms in the sum have contributions: $k=i, l=j$ and $k=j,l=i$. So\n",
    "\n",
    "$$\\frac{\\partial^2}{\\partial x_i \\partial x_j} f(x) = \\frac{1}{2} \\frac{\\partial^2}{\\partial x_i \\partial x_j} (x_i A_{ij} x_j + x_j A_{ji} x_i)  = \\frac{1}{2}(A_{ij} + A_{ji})$$\n",
    "\n",
    "Since $A$ is symmetric, so $A_{ij} = A_{ji}$. So:\n",
    "\n",
    "$$\\frac{\\partial^2}{\\partial x_i \\partial x_j} f(x) =A_{ij}$$\n",
    "\n",
    "So\n",
    "\n",
    "$$\\nabla^2 f(x) = A$$\n",
    "\n",
    "(d)\n",
    "$$\\frac{\\partial}{\\partial x_i} f(x) = \\frac{\\partial}{\\partial x_i} g(a^T x) = g'(a^T x)\\frac{\\partial}{\\partial x_i} \\sum_{j=1}^n (a_j x_j)= g'(a^T x) \\sum_{j=1}^n a_j \\delta_{ij} = g'(a^T x) a_i$$\n",
    "So\n",
    "$$\\nabla f(x) = g'(a^T x) a$$\n",
    "\n",
    "Then we calculate $\\nabla^2 f(x)$. The result is a matrix, so let's calculate the element on $i_{th}$ row and $j_{th}$ column.\n",
    "\n",
    "$$\n",
    "\\begin{align}\n",
    "(\\nabla^2 f(x))_{ij} &= \\frac{\\partial^2}{\\partial x_i \\partial x_j} g(a^T x)\n",
    "\\\\\n",
    "&= \\frac{\\partial}{\\partial x_i} g'(a^T x) a_j\n",
    "\\\\\n",
    "&= a_i a_j g''(a^T x)\n",
    "\\end{align}\n",
    "$$\n",
    "\n",
    "Therefore\n",
    "\n",
    "$$\\nabla^2 f(x) = aa^T g''(a^T x)$$"
   ]
  },
  {
   "cell_type": "markdown",
   "id": "8b20efae-df98-46b1-b944-a28c59c54806",
   "metadata": {},
   "source": [
    "2\n",
    "\n",
    "(a)\n",
    "\n",
    "For any vector $x$, we have\n",
    "\n",
    "$$x^T A x = x^T zz^T x = (z^T x)^T z^T x \\geq 0$$\n",
    "\n",
    "Therefore $A$ is positive semidefinite.\n",
    "\n",
    "(b)\n",
    "\n",
    "If $x$ is in the null-space of $A$, we must have: $A x = 0$, which means $zz^T x = 0$. Therefore, $x^T zz^T x= 0$. So $(z^T x)^Tz^T x= 0$. So $z^T x = 0$.\n",
    "\n",
    "So the null-space of $A$ is a set of all vectors $x$ such that $z^T x = 0$.\n",
    "\n",
    "It is easy to see the rank of $A$ is at most 1, because any two rows are linearly dependent: The $i_{th}$ row is $z_i z^T$, and the $j_{th}$ row is $z_j z^T$.\n",
    "\n",
    "Since $z$ is a non-zero vector, there is at least one element in the diagonal one $A$ that is not zero. So the rank of $A$ is at least 1.\n",
    "\n",
    "Therefore, the rank of $A$ is 1.\n",
    "\n",
    "(c)\n",
    "\n",
    "Yes. \n",
    "\n",
    "First we verify that $BAB^T$ is symmetric:\n",
    "\n",
    "$$(BAB^T)^T = BA^TB^T = BAB^T$$\n",
    "\n",
    "Then, for any vector $x$, we have\n",
    "\n",
    "$$x^T BAB^T x = (B^T x)^T A B^T x = y^TAy$$\n",
    "\n",
    "where we let $y = B^T x$. \n",
    "\n",
    "Since $A$ is PSD, then for any $y$, we have $y^T A y \\geq 0$. So $x^T BAB^T x \\geq 0$. Therefore $BAB^T$ is PSD."
   ]
  },
  {
   "cell_type": "markdown",
   "id": "6ad95cb9-6f1f-4941-8337-c60a8b2e9b8b",
   "metadata": {},
   "source": [
    "3\n",
    "\n",
    "(a)\n",
    "\n",
    "From $A=T\\Lambda T^{-1}$ we have $AT = T\\Lambda$. So\n",
    "$$A(t^{(1)},...,t^{(n)})= (t^{(1)},...,t^{(n)})\\Lambda$$\n",
    "\n",
    "For $i_{th}$ column, we have\n",
    "\n",
    "$$At^{(i)} = \\lambda_i t^{(i)} $$\n",
    "\n",
    "(b)\n",
    "\n",
    "We use $U^T = U^{-1}$, then it reduces to (a).\n",
    "\n",
    "(c)\n",
    "\n",
    "Since A is PSD, then for any $x$ we have\n",
    "\n",
    "$$x^T A x \\geq 0$$\n",
    "\n",
    "Since $A$ is PSD, $A=A^T$. According to the spectral theorem, there exists an orthogonal matrix $U$ such that:\n",
    "\n",
    "$$A=U\\Lambda U^T$$\n",
    "\n",
    "which means \n",
    "\n",
    "$$x^T U\\Lambda U^T x \\geq 0$$ \n",
    "\n",
    "let $y = U^T x$, then $y^T \\Lambda y \\geq 0$ for any $y$.\n",
    "\n",
    "Let $y = (0,...,1, ...,0)^T$ (only $y_i = 1$), we have $\\lambda_i \\geq 0$."
   ]
  }
 ],
 "metadata": {
  "kernelspec": {
   "display_name": "Python 3 (ipykernel)",
   "language": "python",
   "name": "python3"
  },
  "language_info": {
   "codemirror_mode": {
    "name": "ipython",
    "version": 3
   },
   "file_extension": ".py",
   "mimetype": "text/x-python",
   "name": "python",
   "nbconvert_exporter": "python",
   "pygments_lexer": "ipython3",
   "version": "3.12.6"
  }
 },
 "nbformat": 4,
 "nbformat_minor": 5
}
