{
 "cells": [
  {
   "cell_type": "markdown",
   "id": "5236a51a-8980-4e8c-96f1-cfb369c80205",
   "metadata": {},
   "source": [
    "(a)\n",
    "\n",
    "We know that\n",
    "\n",
    "$$p(\\theta|x,y)p(y|x)p(x)=p(x,y,\\theta) = p(y|x,\\theta)p(\\theta|x)p(x)$$\n",
    "\n",
    "So\n",
    "\n",
    "$$p(\\theta|x,y) = \\frac{p(y|x,\\theta)p(\\theta|x)}{p(y|x)}$$\n",
    "\n",
    "Therefore,\n",
    "\n",
    "$$\n",
    "\\begin{align}\n",
    "\\theta_{MAP} &= \\arg \\max_\\theta p(\\theta|x,y)\n",
    "\\\\\n",
    "&= \\arg \\max_\\theta \\frac{p(y|x,\\theta)p(\\theta|x)}{p(y|x)}\n",
    "\\\\\n",
    "&= \\arg \\max_\\theta p(y|x,\\theta)p(\\theta|x)\n",
    "\\\\\n",
    "&= \\arg \\max_\\theta p(y|x,\\theta)p(\\theta)\n",
    "\\end{align}\n",
    "$$\n",
    "\n",
    "(b)\n",
    "\n",
    "Start from the result in (a), we have\n",
    "\n",
    "$$\n",
    "\\begin{align}\n",
    "\\theta_{MAP}\n",
    "&= \\arg \\max_\\theta p(y|x,\\theta)p(\\theta)\n",
    "\\\\\n",
    "&= \\arg \\max_\\theta \\ln[p(y|x,\\theta)p(\\theta)]\n",
    "\\\\\n",
    "&= \\arg \\min_\\theta -\\ln[p(y|x,\\theta)p(\\theta)]\n",
    "\\\\\n",
    "&= \\arg \\min_\\theta -\\ln p(y|x,\\theta) - \\ln p(\\theta)\n",
    "\\\\\n",
    "&= \\arg \\min_\\theta -\\ln p(y|x,\\theta) - \\ln \\frac{1}{(2\\pi)^{n/2}\\eta} e^{-\\frac{||\\theta||_2^2}{2\\eta^2}}\n",
    "\\\\\n",
    "&= \\arg \\min_\\theta -\\ln p(y|x,\\theta) +\\frac{||\\theta||_2^2}{2\\eta^2}\n",
    "\\end{align}\n",
    "$$\n",
    "\n",
    "so\n",
    "\n",
    "$$\\lambda = \\frac{1}{2\\eta^2}$$"
   ]
  },
  {
   "cell_type": "markdown",
   "id": "601487f1-d5be-49d0-ab66-7ec22c50ff1e",
   "metadata": {},
   "source": [
    "(c)\n",
    "\n",
    "We know that \n",
    "\n",
    "$$p(y|x,\\theta) \\sim N(\\theta^T x, \\sigma^2) = \\frac{1}{\\sqrt{2\\pi}\\sigma}\\exp[-\\frac{(y-\\theta^Tx)^2}{2\\sigma^2}]$$\n",
    "\n",
    "Plug in the result of (b), we have\n",
    "\n",
    "$$\n",
    "\\begin{align}\n",
    "\\theta_{MAP} \n",
    "&= \\arg \\min_\\theta \\sum_{i=1}^m \\frac{(y^{(i)}-\\theta^Tx^{(i)})^2}{2\\sigma^2} +\\lambda||\\theta||_2^2\n",
    "\\\\\n",
    "&= \\arg \\min_\\theta \\frac{1}{2\\sigma^2} (X\\theta -y)^T(X\\theta -y) +\\frac{1}{2\\eta^2} \\theta^T \\theta\n",
    "\\end{align}$$\n",
    "\n",
    "The way to calculate $\\theta_{MAP}$ is to take the gradient with respect to $\\theta$ and set the gradient to 0.\n",
    "\n",
    "$$\\nabla_\\theta [\\frac{1}{2\\sigma^2} (X\\theta -y)^T(X\\theta -y) +\\frac{1}{2\\eta^2} \\theta^T \\theta] = \\frac{1}{\\sigma^2}(X^T X \\theta - X^T y) + \\frac{1}{\\eta^2} \\theta$$\n",
    "\n",
    "Setting the derivative above to 0, we can solve for $\\theta$, which is just $\\theta_{MAP}$:\n",
    "\n",
    "$$\\theta_{MAP} = (X^TX +\\frac{\\sigma^2}{\\eta^2} I)^{-1}X^Ty$$"
   ]
  },
  {
   "cell_type": "markdown",
   "id": "d6341390-2f49-43a4-9a8e-ca912f288ce8",
   "metadata": {},
   "source": [
    "(d)\n",
    "\n",
    "We start from the result in (a)\n",
    "\n",
    "$$\\theta_{MAP} =\\arg \\max_\\theta p(y|x,\\theta)p(\\theta)$$\n",
    "\n",
    "Or \n",
    "\n",
    "$$\\theta_{MAP} =\\arg \\max_\\theta \\ln (p(y|x,\\theta)p(\\theta)) = \\arg \\min_\\theta (-\\ln p(y|x,\\theta) -\\ln p(\\theta))$$\n",
    "\n",
    "Then we plug in\n",
    "\n",
    "$$p(y|x,\\theta) \\sim N(\\theta^T x, \\sigma^2) = \\frac{1}{\\sqrt{2\\pi}\\sigma}\\exp[-\\frac{(y-\\theta^Tx)^2}{2\\sigma^2}]$$\n",
    "\n",
    "and the Laplace prior\n",
    "\n",
    "$$p(\\theta) = \\frac{1}{(2b)^m} \\exp(-\\frac{||\\theta||_1}{b})$$\n",
    "\n",
    "We then have\n",
    "\n",
    "$$\n",
    "\\begin{align}\n",
    "\\theta_{MAP} &=\\arg \\min_\\theta (-\\ln p(y|x,\\theta) -\\ln p(\\theta))\n",
    "\\\\\n",
    "&=\\arg \\min_\\theta (\\sum_{i=1}^m \\frac{(y^{(i)}-\\theta^Tx^{(i)})^2}{2\\sigma^2} + \\frac{||\\theta||_1}{b})\n",
    "\\\\\n",
    "&=\\arg \\min_\\theta (\\frac{||X\\theta - y||_2^2}{2\\sigma^2} + \\frac{||\\theta||_1}{b})\n",
    "\\\\\n",
    "&=\\arg \\min_\\theta (||X\\theta - y||_2^2 +  \\frac{2\\sigma^2}{b}||\\theta||_1)\n",
    "\\\\\n",
    "&=\\arg \\min_\\theta J(\\theta)\n",
    "\\end{align}$$\n",
    "\n",
    "where\n",
    "$$J(\\theta) = ||X\\theta - y||_2^2 +  \\frac{2\\sigma^2}{b}||\\theta||_1 $$\n",
    "\n",
    "We can see that \n",
    "\n",
    "$$\\gamma = \\frac{2\\sigma^2}{b}$$"
   ]
  }
 ],
 "metadata": {
  "kernelspec": {
   "display_name": "Python 3 (ipykernel)",
   "language": "python",
   "name": "python3"
  },
  "language_info": {
   "codemirror_mode": {
    "name": "ipython",
    "version": 3
   },
   "file_extension": ".py",
   "mimetype": "text/x-python",
   "name": "python",
   "nbconvert_exporter": "python",
   "pygments_lexer": "ipython3",
   "version": "3.12.6"
  }
 },
 "nbformat": 4,
 "nbformat_minor": 5
}
